ulib/LowStar.Buffer.fst
@@ -14,7 +14,7 @@ noeq
 type buffer' (a: Type0) : Type0 =
 | Null
 | Buffer:
-  (max_length: U32.t { U32.v max_length > 0 } ) ->
+  (max_length: U32.t ) ->
   (content: HST.reference (vec a (U32.v max_length))) ->
   (idx: U32.t) ->
   (length: U32.t { U32.v idx + U32.v length <= U32.v max_length } ) ->
@@ -1125,6 +1125,7 @@ let freeable' (#a: Type) (b: buffer a) : GTot Type0 =
   (not (g_is_null b)) /\
   HS.is_mm (Buffer?.content b) /\
   HST.is_eternal_region (frameOf b) /\
+  U32.v (Buffer?.max_length b) > 0 /\
   Buffer?.idx b == 0ul /\
   Buffer?.length b == Buffer?.max_length b
 
